src/tls/Negotiation.fst
@@ -439,10 +439,12 @@ let computeOffer r cfg resume nonce ks pskinfo =
     match pskinfo with
     | (_, i) :: _ -> i.allow_early_data // Must be the first PSK
     | _ -> false in
+  (* Moved to application callback
   let qp =
     match cfg.quic_parameters with
     | Some (qv::_, qp) -> Some (QuicParametersClient qv qp)
     | _ -> None in
+  *)
   let extensions =
     Extensions.prepareExtensions
       cfg.min_version
@@ -450,7 +452,7 @@ let computeOffer r cfg resume nonce ks pskinfo =
       cfg.cipher_suites
       cfg.peer_name
       cfg.alpn
-      qp
+      // qp
       cfg.extended_master_secret
       cfg.safe_renegotiation
       (compatible_psk && Some? cfg.max_early_data)
@@ -706,14 +708,14 @@ let client_HelloRetryRequest #region (ns:t region Client) hrr (s:option share) =
     let ext' = TLSConstants.choose_aux s choose_extension (Some?.v offer.ch_extensions) in
 
     // Echo the cookie for QUIC stateless retry
-    let ext' = match List.Tot.find Extensions.E_cookie? el with
-      | Some cookie -> cookie :: ext'
-      | None -> ext' in
+    let ext', no_cookie = match List.Tot.find Extensions.E_cookie? el with
+      | Some cookie -> cookie :: ext', false
+      | None -> ext', true in
 
     if sid <> offer.ch_sessionID then
       Error(AD_illegal_parameter, "mismatched session ID in HelloRetryRequest")
-    else if None? (group_of_hrr hrr) && None? ns.cfg.quic_parameters then
-      Error(AD_illegal_parameter, "only keyShare-based HRR is supported on client")
+    else if None? (group_of_hrr hrr) && no_cookie then
+      Error(AD_illegal_parameter, "received a HRR that would yield the same ClientHello")
     else
      begin
       let offer' = {offer with ch_extensions = Some ext'} in
@@ -1226,10 +1228,15 @@ let rec register_shares (l:list pre_share)
   | [] -> []
   | (| g, gx |) :: t -> (| g, CommonDH.register #g gx |) :: (register_shares t)
 
+// For application-handled extensions set by nego callback,
+// such as QUIC transport parameters
+type extra_ext = // list (e:Extensions.extension{E_unknown_extension? e})
+  list Extensions.extension
+
 //17-03-30 still missing a few for servers.
 type serverMode =
   | ServerHelloRetryRequest: hrr -> serverMode
-  | ServerMode: mode -> certNego -> serverMode
+  | ServerMode: mode -> certNego -> extra_ext -> serverMode
 
 let get_sni (o:offer) : bytes =
   match find_client_extension Extensions.E_server_name? o with
@@ -1271,7 +1278,6 @@ let computeServerMode cfg co serverRandom =
         hrr_extensions = [
           Extensions.E_supported_versions (Extensions.ServerPV TLS_1p3);
           Extensions.E_key_share (CommonDH.HRRKeyShare ng);
-          Extensions.E_cookie (CoreCrypto.random 32)
         ]; } in
       Correct(ServerHelloRetryRequest hrr)
     | Correct ((PSK_EDH j ogx cs)::_, _) ->
@@ -1289,7 +1295,7 @@ let computeServerMode cfg co serverRandom =
         None // TODO: n_client_cert_request
         None
         ogx)
-      None)) // No cert
+      None [])) // No cert
     | Correct ((JUST_EDH gx cs) :: _, _) ->
       (trace "Negotiated Pure EDH key exchange";
       let Some (cert, sa) = scert in
@@ -1310,7 +1316,7 @@ let computeServerMode cfg co serverRandom =
           None // TODO: n_client_cert_request
           (Some (Cert.chain_up schain, sa))
           (Some gx))
-        scert))
+        scert []))
     end
   | Correct pv ->
     let valid_ticket =
@@ -1335,7 +1341,7 @@ let computeServerMode cfg co serverRandom =
         None
         None
         None
-        None) None)
+        None) None [])
     | _ ->
       // Make sure NullCompression is offered
       if not (List.Tot.mem NullCompression co.ch_compressions)
@@ -1368,7 +1374,7 @@ let computeServerMode cfg co serverRandom =
                 None
                 (Some (Cert.chain_up schain, sa))
                 None) // no client key share yet for 1.2
-              (Some(cert, sa))
+              (Some(cert, sa)) []
             ))
 
 private
@@ -1400,9 +1406,9 @@ let aux_extension_ok (o1, hrr) (e:Extensions.extension) =
             //(extensionBytes e) = (extensionBytes e'))
 
 val server_ClientHello: #region:rgn -> t region Server ->
-  HandshakeMessages.ch ->
+  HandshakeMessages.ch -> log:HandshakeLog.t ->
   St (result serverMode)
-let server_ClientHello #region ns offer =
+let server_ClientHello #region ns offer log =
   trace ("offered client extensions "^string_of_option_extensions offer.ch_extensions);
   trace ("offered cipher suites "^(string_of_ciphersuites offer.ch_cipher_suites));
   trace (match (offered_versions TLS_1p0 offer) with
@@ -1428,47 +1434,93 @@ let server_ClientHello #region ns offer =
         Error z
       | Correct (ServerHelloRetryRequest hrr) ->
         Error(AD_illegal_parameter, "client sent the same hello in response to hello retry")
-      | Correct(ServerMode m cert) ->
+      | Correct (ServerMode m cert _) ->
         trace ("negotiated after HRR "^string_of_pv m.n_protocol_version^" "^string_of_ciphersuite m.n_cipher_suite);
-        HST.op_Colon_Equals ns.state (S_ClientHello m cert);
-        sm
+        let nego_cb = ns.cfg.nego_callback in
+        let unk_ext = (* List.Tot.filter Extensions.E_unknown_extension? *) o2.ch_extensions in
+        let ext_bytes = HandshakeMessages.optionExtensionsBytes unk_ext in
+        match nego_cb.server_nego nego_cb.server_nego_context m.n_protocol_version ext_bytes (Some empty_bytes) with
+        | Nego_accept sexts ->
+          (match Extensions.parseOptExtensions Extensions.EM_ServerHello sexts with
+          | Error z -> Error (AD_internal_error, "server negotiation callback returned ill-formatted extra extensions")
+          | Correct (el, _) ->
+            let el = match el with | None -> [] | Some l -> l in
+            HST.op_Colon_Equals ns.state (S_ClientHello m cert);
+            Correct (ServerMode m cert el))
+        | _ ->
+          trace ("Application requested to abort the handshake after internal HRR.");
+          Error (AD_handshake_failure, "application aborted the handshake by callback")
     else
       Error(AD_illegal_parameter, "Inconsistant parameters between first and second client hello")
   | S_Init _ ->
     let sm = computeServerMode ns.cfg offer ns.nonce in
+    let previous_cookie = // for stateless HRR
+      match find_cookie offer with
+      | None -> None
+      | Some c ->
+        match Ticket.check_cookie c with
+        | None -> trace ("WARNING: ignorning invalid cookie "^(hex_of_bytes c)); None
+        | Some (hrr, digest, extra) ->
+          trace ("Loading cookie "^(hex_of_bytes c));
+          let hrr = { hrr with hrr_extensions =
+            (Extensions.E_cookie c) :: hrr.hrr_extensions; } in
+          // Overwrite the current transcript digest with values from cookie
+          HandshakeLog.load_stateless_cookie log hrr digest;
+          Some extra // for the server nego callback
+      in
     match sm with
     | Error z ->
       trace ("negotiation failed: "^string_of_error z);
       Error z
     | Correct (ServerHelloRetryRequest hrr) ->
+      // Internal HRR caused by group negotiation
+      // We do not invoke the server nego callback in this case
       // record the initial offer and return the HRR to HS
+      let ha = verifyDataHashAlg_of_ciphersuite hrr.hrr_cipher_suite in
+      let digest = HandshakeLog.hash_tag #ha log in
+      let cookie = Ticket.create_cookie hrr digest empty_bytes in
+      let hrr = { hrr with hrr_extensions =
+        (Extensions.E_cookie cookie) :: hrr.hrr_extensions; } in
       HST.op_Colon_Equals ns.state (S_HRR offer hrr);
       sm
-    | Correct (ServerMode m cert) ->
-      // Forcing HRR for source address validation
-      if ns.cfg.offer_shares = [] then
+    | Correct (ServerMode m cert _) ->
+      let nego_cb = ns.cfg.nego_callback in
+      let unk_ext = (* List.Tot.filter Extensions.E_unknown_extension? *) offer.ch_extensions in
+      let ext_bytes = HandshakeMessages.optionExtensionsBytes unk_ext in
+      match nego_cb.server_nego nego_cb.server_nego_context m.n_protocol_version ext_bytes previous_cookie with
+      | Nego_abort ->
+        trace ("Application requested to abort the handshake.");
+        Error (AD_handshake_failure, "application aborted the handshake by callback")
+      | Nego_retry cextra ->
         let hrr = ({
           hrr_sessionID = offer.ch_sessionID;
           hrr_cipher_suite = m.n_cipher_suite;
           hrr_extensions = [
             Extensions.E_supported_versions (Extensions.ServerPV TLS_1p3);
-            Extensions.E_cookie (CoreCrypto.random 32)
           ]}) in
+        let ha = verifyDataHashAlg_of_ciphersuite hrr.hrr_cipher_suite in
+        let digest = HandshakeLog.hash_tag #ha log in
+        let cookie = Ticket.create_cookie hrr digest cextra in
+        let hrr = { hrr with hrr_extensions =
+          (Extensions.E_cookie cookie) :: hrr.hrr_extensions; } in
         ns.state := (S_HRR offer hrr);
         Correct (ServerHelloRetryRequest hrr)
-      else
-       begin
+      | Nego_accept sext ->
         trace ("negotiated "^string_of_pv m.n_protocol_version^" "^string_of_ciphersuite m.n_cipher_suite);
-        ns.state := (S_ClientHello m cert);
-        sm
-       end
+        match Extensions.parseOptExtensions Extensions.EM_ServerHello sext with
+        | Error z -> Error (AD_internal_error, "server negotiation callback returned ill-formatted extra extensions")
+        | Correct (el, _) ->
+          let el = match el with | None -> [] | Some l -> l in
+          ns.state := S_ClientHello m cert;
+          Correct (ServerMode m cert el)
 
 let share_of_serverKeyShare (ks:CommonDH.serverKeyShare) : share =
   let CommonDH.Share g gy = ks in (| g, gy |)
 
-val server_ServerShare: #region:rgn -> t region Server -> option CommonDH.serverKeyShare  ->
+val server_ServerShare: #region:rgn -> t region Server ->
+  option CommonDH.serverKeyShare -> extra_ext ->
   St (result mode)
-let server_ServerShare #region ns ks =
+let server_ServerShare #region ns ks app_exts =
   match HST.op_Bang ns.state with
   | S_ClientHello mode cert ->
     let cexts = mode.n_offer.ch_extensions in
@@ -1488,6 +1540,12 @@ let server_ServerShare #region ns ks =
     | Correct sexts ->
       begin
       trace ("including server extensions (SH + EE) " ^ string_of_option_extensions sexts);
+      let sexts = match sexts with
+        | Some el ->
+          trace ("extra extensions from application callback: "^string_of_extensions app_exts);
+          Some (el @ app_exts)
+        | _ -> sexts
+        in
       let mode = Mode
         mode.n_offer
         mode.n_hrr
